src/examples/lockfree/treiber.v
@@ -1,5 +1,5 @@
 From iris.base_logic.lib Require Export ghost_map gen_heap.
-From iris.algebra Require Import numbers auth list gset.
+From iris.algebra Require Import numbers auth list gset gmultiset.
 
 From irisfit.program_logic Require Import wpc_logatom.
 From irisfit.program_logic Require Import wp_alloc wp_store wp_call wp_store wp_protected wp_cas wp_load wp_clean wp_free wp_call_prim.
@@ -30,6 +30,11 @@ Definition pop : val :=
       let: "b" := tm_cas "s" 0 "h" "h'" in
       if: "b" then let: "v" := "h".[0] in tm_exit ;; "v" else tm_exit ;; "self" [["s"]].
 
+Definition is_empty : val :=
+  λ: [["s"]],
+    let: "l" := "s".[0] in
+    "l" '== val_unit.
+
 (******************************************************************************)
 (* The cmras we need. *)
 
@@ -41,11 +46,11 @@ Notation elem := (val * (Qp * Qz))%type.
 
 Class stackG Σ :=
   StackG {
-      stack_bonesG : inG Σ (authUR (gsetUR locO));
-      stack_protectG : ghost_mapG Σ nat (loc*loc);
+      stack_cellsG : inG Σ (authUR (gsetUR locO));
+      stack_protectG : inG Σ (authUR (gmultiset  (loc*loc)));
     }.
 
-Local Existing Instances stack_bonesG stack_protectG.
+Local Existing Instances stack_cellsG stack_protectG.
 
 Record gstack := mk_gs { gb : gname; gp : gname }.
 Global Instance gstack_eq_dec : EqDecision gstack.
@@ -71,100 +76,111 @@ Context `{interpGS0 Σ, stackG Σ}.
   deallocate (thanks to GC-less sections) all the private cells
   pointing to it, and then deallocate the cell.
 
-  To allow for private cells, we use a mechanism of "bones".
-  Inner cells are bones. Each bone is either deallocated or pointed
+  To allow for private cells, we use a mechanism of "cells".
+  Each cell is either deallocated or pointed
   by some locations.
   These locations appears in the codomain of a ghost protection map.
  *)
 
-Definition isbone  (γ:gname) (l:loc) : iProp Σ :=
+Definition iscell  (γ:gname) (l:loc) : iProp Σ :=
   own γ (◯ {[l]}).
 
-Definition protect γ v l : iProp Σ :=
-  isbone γ v ∗ sizeof l 2 ∗
-  ((l ↤ ∅ ∗ l ⟸ ∅) ∨ († v ∗ †l ∗ ♢2)).
+Definition volatile (γ:gname) (l:loc) Φ : iProp Σ :=
+  ((sizeof l 2 ∗ l ↤ ∅ ∗ l ⟸ ∅) ∨ (Φ ∗ †l ∗ ♢2)).
 
-Definition protection (γ:gname) (M:gmap nat (loc*loc)) : iProp Σ :=
-  [∗ map] π ↦ x ∈ M, protect γ x.1 x.2.
+(* c is an inner cell, l a private loc *)
+Definition protect (γ:gname) (c:loc) (l:loc) : iProp Σ :=
+  volatile γ l (†c)%I.
 
-Definition stamped (v:loc) (L:gmultiset loc) (M:gmap nat (loc*loc)) :=
-  forall l', l' ∈ L <-> exists π, M !! π = Some (v,l').
+Definition outsiders (γ:gname) (M:gmultiset (loc*loc)) : iProp Σ :=
+  [∗ mset] x ∈ M, protect γ x.1 x.2.
 
-Definition nodup `{Countable A} (X:gmultiset A) :=
-  forall l, multiplicity l X <= 1.
+Definition stamped (v:loc) (L:gmultiset loc) (M:gmultiset (loc*loc)) :=
+  forall l', multiplicity l' L <= multiplicity (v,l') M.
 
-Definition bone M l : iProp Σ :=
+Definition cell M l : iProp Σ :=
   †l ∨
-  (∃ L, l ↤{1/2} (smultiset.of_gmultiset L) ∗
-        ⌜stamped l L M /\ nodup L⌝).
+  (∃ L, l ↤{1/2} (smultiset.of_gmultiset L) ∗ ⌜stamped l L M⌝).
 
-Definition bones (γ:gname) (M:gmap nat (loc*loc)) : iProp Σ :=
+Definition cells (γ:gname) (M:gmultiset (loc*loc)) : iProp Σ :=
   ∃ (A:gset loc),
-    own γ (● A) ∗ [∗ set] l ∈ A, bone M l.
+    own γ (● A) ∗ [∗ set] l ∈ A, cell M l.
 
-Fixpoint spine (γ:gname) (xs:list (val*(Qp*Qz))) (v:val) : iProp Σ :=
+Definition reg (γ:gname) (v:val) : iProp Σ :=
+  ⌜v=val_unit⌝ ∨ (∃ l, ⌜v=val_loc l⌝ ∗ iscell γ l).
+
+Fixpoint innerList (γ:gname) (xs:list (val*(Qp*Qz))) (v:val) : iProp Σ :=
   match xs with
   | nil => ⌜v=val_unit⌝
   | (x,(p,q))::xs =>
       ∃ l v', ⌜v=val_loc l⌝ ∗
-      l ↦□ [x; v'] ∗ l ⟸ ∅ ∗ isbone γ l ∗
-      (* One half of pointedby here, the other half in bones. *)
+      l ↦□ [x; v'] ∗ v' ⟸? ∅ ∗ reg γ v' ∗
+      (* One half of pointedby here, the other half in cells. *)
       v' ↤?{1/2} {[+l+]} ∗ x ⟸?{p} ∅ ∗ x ↤?{q} {[+l+]} ∗
-      spine γ xs v' end.
+      innerList γ xs v' end.
 
-Global Instance spine_timeless γ xs v : Timeless (spine γ xs v).
+Local Instance innerList_timeless γ xs v : Timeless (innerList γ xs v).
 Proof. revert v; induction xs as [|(?&?&?)]; apply _. Qed.
 
-Definition phys_stack γ (s:loc) (xs:list elem) : iProp Σ :=
-  †s ∨ ∃ v, s ↦ [v] ∗ v ↤?{1/2} {[+s+]} ∗ spine γ xs v.
-
-Definition visbone (γ:gname) (v:val) : iProp Σ :=
-  ⌜v=val_unit⌝ ∨ (∃ l, ⌜v=val_loc l⌝ ∗ isbone γ l).
-
-Lemma spine_visbone γ xs v :
-  spine γ xs v -∗ visbone γ v.
-Proof.
-  destruct xs as [|(?&?&?)].
-  { iIntros "->". by iLeft. }
-  { iIntros "[%[% (->&?&?&?&_)]]". iRight. iExists _. by iFrame. }
-Qed.
-
-Definition kindofinj (M:gmap nat (loc*loc)) :=
-  forall i1 i2 v1 v2 l,
-    M !! i1 = Some (v1,l) ->
-    M !! i2 = Some (v2,l) ->
-    i1 = i2.
+Definition inner γ (s:loc) (xs:list elem) : iProp Σ :=
+  ∃ v, s ↦ [v] ∗ v ⟸? ∅ ∗ v ↤?{1/2} {[+s+]} ∗ reg γ v ∗ innerList γ xs v.
 
 Definition nm := nroot.@"treiber".
 
 Definition stack (s:loc) (xs:list elem) : iProp Σ :=
-  ∃ (g:gstack) (M:gmap nat (loc*loc)),
+  ∃ (g:gstack) (M:gmultiset (loc*loc)),
     meta s nm g ∗
-    ⌜kindofinj M⌝ ∗
-    phys_stack g.(gb) s xs ∗
-    ghost_map_auth g.(gp) 1 M ∗
-    protection g.(gb) M ∗
-    bones g.(gb) M.
+    inner g.(gb) s xs ∗
+    own g.(gp) (● M) ∗
+    outsiders g.(gb) M ∗
+    cells g.(gb) M.
 
 Lemma open_stack_inv_meta s g xs :
   meta s nm g -∗
   stack s xs -∗
-  ∃ (M:gmap nat (loc*loc)),
-    ⌜kindofinj M⌝ ∗
-    phys_stack g.(gb) s xs ∗
-    ghost_map_auth g.(gp) 1 M ∗
-    protection g.(gb) M ∗
-    bones g.(gb) M.
+  ∃ (M:gmultiset (loc*loc)),
+    inner g.(gb) s xs ∗
+    own g.(gp) (● M) ∗
+    outsiders g.(gb) M ∗
+    cells g.(gb) M.
 Proof.
   iIntros "Hmeta (%&%&Hmeta'&?)".
   iDestruct (meta_agree with "Hmeta Hmeta'") as "->".
   iExists _. by iFrame.
 Qed.
 
+Lemma is_empty_spec π xs s :
+  CODE (is_empty [[s]])
+  TID π
+  SOUV {[s]}
+  PRE  (stack s xs)
+  POST (fun (b:bool) => ⌜b <-> xs=nil⌝ ∗ stack s xs).
+Proof.
+  iIntros "Hs".
+  wpc_call. wpc_let_empty.
+  iDestruct "Hs" as "[%g [%M (#Hmeta&I1&I2&I3&I4)]]".
+
+  iApply wpc_split_ctx. iIntros (X HX) "HPBT".
+  assert (is_Some (X !! s)) as (p&Hp).
+  { apply elem_of_dom. set_solver. }
+  iDestruct (PBT_borrow_pbt with "[$]") as "(Hp&Hback)". done.
+  iDestruct "I1" as "[%h (S1&S2&S3&S4&S5)]".
+  iSpecialize ("Hback" with "[$]").
+  destruct xs as [|(?&?&?)]; simpl.
+  { iDestruct "S5" as "->". wpc_load. iSteps. wpc_call_prim. iSteps. }
+  { iDestruct "S5" as "(%&%&->&?)".
+    wpc_load. iIntros "(?&?)". iApply wpc_postpone.
+    wpc_call_prim. pclean l. wpc_val. iSplitR; first done. iExists g,M. iFrame "#∗".
+    iExists _. iFrame. simpl. iSteps. }
+  Unshelve. all:exact inhabitant.
+Qed.
+
 Lemma create_spec π :
-  ♢1 -∗
-  wpc ⊤ π (Some ∅) (create [[]])%T
-    (fun (s:loc) => stack s [] ∗ s ⟸ {[π]} ∗ s ↤ ∅).
+  CODE (create [[]])
+  TID π
+  SOUV ∅
+  PRE (♢1)
+  POST (fun (s:loc) => stack s [] ∗ s ⟸ {[π]} ∗ s ↤ ∅).
 Proof.
   iIntros.
   wpc_call.
@@ -173,83 +189,81 @@ Proof.
   wpc_alloc.
   iIntros (s) "(?&X1&X2&?)".
 
-  iMod (own_alloc (● ∅)) as "[%γ2 H2]".
+  iMod (own_alloc (● (∅:gset loc))) as "[%γ2 H2]".
   { by apply auth_auth_valid. }
 
-  iMod ghost_map_alloc_empty  as "[%γ3 ?]".
+  iMod (own_alloc (● (∅:gmultiset (loc*loc)))) as "[%γ3 H3]".
+  { by apply auth_auth_valid. }
 
   pose (g := mk_gs γ2 γ3).
   iMod (meta_set _ s g nm with "[$]") as "#?". solve_ndisj.
 
   iAssert (stack s nil) with "[-X1 X2]" as "Hs".
-  { iExists _,_. subst g. simpl. iFrame "#∗".
-    iSplitR.
-    { iPureIntro. intros ?????. rewrite lookup_empty. naive_solver. }
+  { iExists _,∅. subst g. simpl. iFrame "#∗". simpl.
     iSplitR "H2".
-    { iRight. iExists _. by iFrame. }
+    { iSmash. }
     iSplitR "H2".
-    { by iApply big_sepM_empty. }
+    { by iApply big_sepMS_empty. }
     { iExists _. iFrame. by iApply big_sepS_empty. } }
 
   wpc_val. iFrame.
 Qed.
 
-Definition reg γ (i:nat) (v:val) (l':loc) : iProp Σ :=
+Definition gelem γ l l' : iProp Σ := own γ (◯ ({[+ (l,l') +]})).
+
+Definition isreg γ (v:val) (l':loc) : iProp Σ :=
   (⌜v=val_unit⌝ ∗ l' ↤ ∅ ∗ l' ⟸ ∅)
-  ∨ (∃ l, ⌜v=val_loc l⌝ ∗ i ↪[γ] (l,l')).
+  ∨ (∃ l, ⌜v=val_loc l⌝ ∗ gelem γ l l').
 
 Lemma register_aux (v:loc) l γ γ' M :
-  isbone γ' v -∗
-  ghost_map_auth γ 1 M -∗
-  protection γ' M -∗
+  (v, l) ∉ M ->
+  iscell γ' v -∗
+  own γ (● M) -∗
+  outsiders γ' M -∗
   sizeof l 2 ∗ l ↤ ∅ ∗ l ⟸ ∅ ==∗
-  ∃ i, ⌜i ∉ dom M⌝ ∗ ghost_map_auth γ 1 (<[i:=(v,l)]>M) ∗ protection γ' (<[i:=(v,l)]>M) ∗ i ↪[γ] (v,l).
+  own γ (● (({[+ (v, l) +]} ⊎ M))) ∗ outsiders γ' ({[+ (v, l) +]} ⊎ M) ∗ gelem γ v l.
 Proof.
-  iIntros  "H1 H2 H3 (?&?&?)". iExists (fresh (dom M)).
-  assert (fresh (dom M) ∉ dom M) by apply is_fresh.
-  iMod (ghost_map_insert (fresh (dom M)) with "[$]") as "(?&?)"; last iFrame.
-  { by apply not_elem_of_dom. }
-  iSplitR. done.
-  iApply big_sepM_insert. by apply not_elem_of_dom.
+  iIntros (?) "H1 H2 H3 (?&?&?)".
+  iMod (own_update with "H2") as "(?&?)".
+  { apply auth_update_alloc.
+    apply gmultiset_local_update with (Y':={[+(v,l)+]}).
+    rewrite right_id_L //. }
+  rewrite comm_L.
+  iFrame. iApply big_sepMS_singleton.
   iFrame. iLeft. by iFrame.
 Qed.
 
-Lemma update_set_bone M M' A :
+Lemma update_set_cell M M' A :
   (forall (l:loc) L, l ∈ A -> stamped l L M -> stamped l L M') ->
-  ([∗ set] y ∈ A, bone M y)%I -∗
-  [∗ set] y ∈ A, bone M' y.
+  ([∗ set] y ∈ A, cell M y)%I -∗
+  [∗ set] y ∈ A, cell M' y.
 Proof.
   iIntros. iApply (big_sepS_impl with "[$]").
-  iModIntro. iIntros (??) "[?|[%(?&%&%)]]".
+  iModIntro. iIntros (??) "[?|[%(?&%)]]".
   by iLeft.
   iRight. iExists _. iFrame. iPureIntro. eauto.
 Qed.
 
-Lemma bones_update γ M M':
+Lemma cells_update γ M M':
   (forall (l:loc) L, stamped l L M -> stamped l L M') ->
-  bones γ M -∗ bones γ M'.
+  cells γ M -∗ cells γ M'.
 Proof.
   iIntros (?) "[% (?&?)]". iExists _. iFrame.
-  iApply (update_set_bone with "[$]"); eauto.
+  iApply (update_set_cell with "[$]"); eauto.
 Qed.
 
-Lemma stamped_insert_fresh (v v':loc) l' L M π :
+Lemma stamped_insert_fresh (v v':loc) l' L M :
   v ≠ v' ->
-  π ∉ dom M ->
   stamped v L M ->
-  stamped v L (<[π:=(v',l')]> M).
+  stamped v L ({[+ (v',l') +]} ⊎ M).
 Proof.
-  intros ? ? E1 l0. rewrite E1. split.
-  { intros (i,Hi). exists i. rewrite lookup_insert_ne //.
-    intros ->. eauto using elem_of_dom. }
-  { intros (i,Hi). rewrite lookup_insert_case in Hi. case_decide; eauto.
-    exfalso. inversion Hi. subst. congruence. }
+  intros ? E l0. specialize (E l0). rewrite multiplicity_disj_union. lia.
 Qed.
 
 Lemma confront_protect_pbt γ l v A :
   l ⟸ A ∗ protect γ v l -∗ False.
 Proof.
-  iIntros "(?&(_&_&[(?&?)|(?&?&?)]))".
+  iIntros "(?&[(_&?&?)|(?&?&?)])".
   { iDestruct (pbt_valid2 with "[$][$]") as "%Hv". exfalso. by vm_compute. }
   { iApply (confront_pbt_dag with "[$]"). }
 Qed.
@@ -258,38 +272,29 @@ Definition vdead v : iProp Σ :=
   ∃ l, ⌜v=val_loc l⌝ ∗ †l.
 
 Lemma register l' γ γ' v M :
-  kindofinj M ->
-  visbone γ' v -∗
+  reg γ' v -∗
   sizeof l' 2 ∗ l' ↤ ∅ ∗ l' ⟸ ∅ -∗
-  bones γ' M -∗
-  ghost_map_auth γ 1 M -∗
-  protection γ' M ==∗
-  ∃ i M', ⌜kindofinj M'⌝ ∗ ghost_map_auth γ 1 M' ∗ protection γ' M' ∗ reg γ i v l' ∗
-  ((vdead v ∗ bones γ' M')
-  ∨  (v ↤?{(1/4)%Qz} ∅ ∗ ((v ↤?{1/4} {[+l'+]}) -∗ bones γ' M'))).
+  cells γ' M -∗
+  own γ (● M) -∗
+  outsiders γ' M ==∗
+  ∃ M', own γ (● M') ∗ outsiders γ' M' ∗ isreg γ v l' ∗
+  ((vdead v ∗ cells γ' M')
+  ∨  (v ↤?{(1/4)%Qz} ∅ ∗ ((v ↤?{1/4} {[+l'+]}) -∗ cells γ' M'))).
 Proof.
-  iIntros (Hk) "#Hb (E1&E2&E3) Hbones H1 H2".
-  iAssert (⌜∀ v i l0, M !! i = Some (v,l0) -> l0 ≠ l'⌝ )%I as "%X".
-  { iIntros (??? HM ->).
-    iDestruct (big_sepM_lookup with "[$]") as "?". apply HM. simpl.
-    iDestruct (confront_protect_pbt with "[$]") as "?". done. }
+  iIntros "#Hb (E1&E2&E3) Hcells H1 H2".
 
   iDestruct "Hb" as "[ -> | [%l (->&?)]]".
-  { iExists 0,M. iFrame. iSmash. }
+  { iSmash. }
 
-  iMod (register_aux with "[$][$][$][$]") as "[%i [%M' (?&?&Hr)]]".
-  iModIntro. iExists i,(<[i:=(l,l')]> M). iFrame.
-  iSplit.
-  { iIntros (????? E1 E2). rewrite lookup_insert_case in E1.
-    case_decide; subst.
-    { rewrite lookup_insert_case in E2. case_decide; subst.
-      { iPureIntro. naive_solver. }
-      { inversion E1. subst. naive_solver. } }
-    { rewrite lookup_insert_case in E2. case_decide; subst.
-      { inversion E2. subst. naive_solver. }
-      { eauto. } } }
+  iAssert (⌜(l, l') ∉ M⌝ )%I as "%X".
+  { iIntros (HM).
+    iDestruct (big_sepMS_elem_of with "[$]") as "?". apply HM. simpl.
+    iDestruct (confront_protect_pbt with "[$]") as "?". done. }
 
-  iDestruct "Hbones" as "[%A (Hba&Hs)]".
+  iMod (register_aux with "[$][$][$][$]") as "(?&?&Hr)". set_solver.
+  iModIntro. iExists ({[+ (l, l') +]} ⊎ M). iFrame.
+
+  iDestruct "Hcells" as "[%A (Hba&Hs)]".
   iDestruct (more_cmras.elem_of_gset with "Hba [$]") as "%".
   replace A with ({[l]} ∪ A ∖ {[l]}).
   2:{ rewrite union_comm_L difference_union_L. set_solver. }
@@ -298,153 +303,127 @@ Proof.
   iSplitL "Hr". iSmash.
   iDestruct "Hs" as "(Hb&Hs)".
 
-  iDestruct "Hb" as "[#?|[% (Hl&(%E2&%E3))]]".
+  iDestruct "Hb" as "[#?|[% (Hl&%E2)]]".
   { iLeft. simpl. iSplitR. iExists _. by iFrame "#".
     iExists _. iFrame. rewrite big_sepS_insert. 2:set_solver.
     iFrame. iFrame "#".
-    iApply (update_set_bone with "[$]").
+    iApply (update_set_cell with "[$]").
     intros. eapply stamped_insert_fresh; eauto. set_solver. }
 
   iRight.
   replace (1 / 2)%Qz with (1/4 + 1/4)%Qz by compute_done.
-  rewrite -(left_id _ _ L).
+  rewrite -(left_id _ _ (of_gmultiset L)).
   iDestruct (mapsfrom_split with "[$]") as "(Hx&?)". 3:done.
   1,2:intros E; exfalso; by vm_compute.
-  { rewrite of_gmultiset_disj_union. done. }
-  rewrite of_gmultiset_empty. iFrame. iIntros.
+  { done. }
+  iFrame. iIntros.
   iExists _. iFrame "Hba". rewrite big_sepS_insert. 2:set_solver.
   iSplitR "Hs".
   { iRight. iExists ({[+ l' +]} ⊎ L). iFrame. iSplitL; last eauto.
     replace (1 / 2)%Qz with (1/4 + 1/4)%Qz by compute_done.
     rewrite of_gmultiset_disj_union of_gmultiset_singleton.
     iApply (mapsfrom_join with "[$][$]").
-    iPureIntro. split_and !; eauto.
-    { intros l0. rewrite gmultiset_elem_of_disj_union gmultiset_elem_of_singleton.
-      destruct_decide (decide (l0=l')); subst.
-      { split. intros _. exists i. rewrite lookup_insert //. eauto. }
-      rewrite E2. split.
-      { intros [|(i',Hi)]; first congruence. exists i'. rewrite lookup_insert_ne //.
-        intros ->. naive_solver. }
-      intros (i',Hi). right. exists i'. rewrite lookup_insert_case in Hi.
-      case_decide; eauto. inversion Hi. done. }
-    { assert (l' ∉ L).
-      { intros R. apply E2 in R. destruct R. naive_solver. }
-      unfold nodup in *. intros. rewrite multiplicity_disj_union.
-      multiset_solver. } }
-  { iApply (update_set_bone with "[$]"). intros.
+    iPureIntro.
+    { intros l0.
+      rewrite !multiplicity_disj_union. specialize (E2 l0). multiset_solver. } }
+  { iApply (update_set_cell with "[$]"). intros.
     eapply stamped_insert_fresh; eauto. set_solver. }
 Qed.
 
 Definition sentenced l n : iProp Σ :=
   (l ⟸ ∅ ∗ l ↤ ∅) ∨ (†l ∗ ♢n).
 
-Lemma stamped_delete (l:loc) M π v (l':loc) L :
+Lemma stamped_delete (l:loc) M v (l':loc) L :
   v ≠ l ->
-  M !! π = Some (v, l') ->
+  (v,l') ∈ M ->
   stamped l L M →
-  stamped l L (delete π M).
+  stamped l L (M ∖ {[+ (v, l') +]}).
 Proof.
-  intros ? ? E l0. rewrite E.
-  split; intros (i,Hi).
-  { exists i. rewrite lookup_delete_ne //. intros ->. naive_solver. }
-  { apply lookup_delete_Some in Hi. naive_solver. }
-Qed.
-
-Lemma kindofinj_delete M π :
-  kindofinj M ->
-  kindofinj (delete π M).
-Proof.
-  intros ??????. rewrite !lookup_delete_Some. naive_solver.
-Qed.
-
-Lemma nodup_remove `{Countable A} (X Y:gmultiset A) :
-  nodup X -> nodup (X ∖ Y).
-Proof.
-  intros E l'. specialize (E l'). rewrite multiplicity_difference. multiset_solver.
+  intros ? ? E l0. rewrite multiplicity_difference.
+  specialize (E l0). multiset_solver.
 Qed.
 
 Definition schrodinger γ M v l : iProp Σ :=
-  ((vdead v ∗ bones γ M ∗ sentenced l 2) ∨
-    l ↤ ∅ ∗ l ⟸ ∅ ∗ v ↤?{1/4}{[+l+]} ∗ (v ↤?{1/4} ∅ -∗ bones γ M )).
+  ((vdead v ∗ cells γ M ∗ sentenced l 2) ∨
+    l ↤ ∅ ∗ l ⟸ ∅ ∗ v ↤?{1/4}{[+l+]} ∗ (v ↤?{1/4} ∅ -∗ cells γ M )).
 
-Lemma unreg l' γ γ' i v M :
-  kindofinj M ->
-  ghost_map_auth γ 1 M ∗
-  protection γ' M ∗
-  bones γ' M ∗
-  visbone γ' v ∗
-  reg γ i v l' =[#]=∗
-  ∃ M', ⌜kindofinj M'⌝ ∗
-        ghost_map_auth γ 1 M' ∗ protection γ' M' ∗ schrodinger γ' M' v l'.
+Lemma unreg l' γ γ' v M :
+  own γ (● M) ∗
+  outsiders γ' M ∗
+  cells γ' M ∗
+  reg γ' v ∗
+  isreg γ v l' =[#]=∗
+  ∃ M', own γ (● M') ∗ outsiders γ' M' ∗ schrodinger γ' M' v l'.
 Proof.
-  iIntros (Hk) "(Ha&Hp&Hb&Hi&Hf)". iIntros.
+  iIntros "(Ha&Hp&Hb&Hi&Hf)". iIntros.
   iDestruct "Hf" as "[ [-> (?&?)] | [%l (->&Hf)]]".
-  { iFrame. iModIntro. iExists _. iFrame "%∗". iSmash. }
-  iDestruct (ghost_map_lookup with "Ha Hf") as "%".
-  iMod (ghost_map_delete with "Ha Hf").
+  { iSmash. }
+  iDestruct (own_valid_2 with "Ha Hf") as "%Hv".
 
-  rewrite /protection big_sepM_delete //.
-  iDestruct "Hp" as "((#?&#?&X)&?)". simpl.
+  apply auth_both_valid_discrete in Hv. destruct Hv as (Hv&_).
+  apply gmultiset_included in Hv.
+  assert ((l, l') ∈ M) by multiset_solver.
+
+  iMod (own_update_2 with "Ha Hf") as "Ha".
+  { apply auth_update_dealloc.
+    apply gmultiset_local_update with (X' := (M ∖ {[+ (l,l') +]})).
+    multiset_solver.  }
+
+  rewrite /outsiders big_sepMS_delete //.
+  iDestruct "Hp" as "(X&?)". simpl.
 
   iDestruct "Hi" as "[%|[%l0 (%Eq&Hf)]]". congruence.
   inversion Eq. subst l0.
-  iDestruct "Hb" as "[% (Ha&Hx)]".
-  iDestruct (more_cmras.elem_of_gset with "Ha Hf") as "%Hv".
+  iDestruct "Hb" as "[% (Hz&Hx)]".
+  iDestruct (more_cmras.elem_of_gset with "Hz Hf") as "%Hv'".
   replace A with ({[l]} ∪ A ∖ {[l]}).
   2:{ rewrite union_comm_L difference_union_L. set_solver. }
   rewrite big_sepS_insert. 2:set_solver. iDestruct "Hx" as "(U&Hx)".
-  iDestruct "U" as "[#?|[%(?&%E2&%E3)]]".
-  { iModIntro. iFrame "#∗".
-    iExists (delete i M). iFrame. iSplitR. eauto using kindofinj_delete.
+  iDestruct "U" as "[#?|[%(Z&%E2)]]".
+  { iModIntro. iFrame "#∗". iExists _. iFrame.
     iLeft. iSplitR. iSmash. iSplitR "X".
-    { iExists _. iFrame "Ha". rewrite big_sepS_insert. 2:set_solver.
-      iSplitR. by iLeft. iApply (update_set_bone with "[$]").
+    { iExists _. iFrame "Hz". rewrite big_sepS_insert. 2:set_solver.
+      iSplitR. by iLeft. iApply (update_set_cell with "[$]").
       { intros. eapply stamped_delete; eauto. set_solver. } }
-    { iDestruct "X" as "[(?&?) | (?&?)]"; [iLeft | iRight]; iFrame "#∗". } }
+    { iDestruct "X" as "[(?&?&?) | (?&?)]"; [iLeft | iRight]; iFrame "#∗". } }
 
-  iDestruct "X" as "[(?&?) | (?&_)]"; last first.
+  iDestruct "X" as "[(?&X&?) | (?&_)]"; last first.
   { iMod (confront_mapsfrom_dag with "[$][$]") as "(?&?)". compute_done.
     done. }
-  iFrame. iModIntro.
-  iExists (delete i M). iFrame "#∗". iSplitR. eauto using kindofinj_delete.
+  iFrame. iModIntro. iExists _. iFrame.
   iRight. iFrame.
-  rewrite (gmultiset_disj_union_difference' l' L).
-  2:{ apply E2. eauto. }
-  replace (1 / 2)%Qz with (1/4 + 1/4)%Qz by compute_done.
-  rewrite of_gmultiset_disj_union.
-  iDestruct (mapsfrom_split with "[$]") as "(?&?)".
-  3,4:done. 1,2:by vm_compute.
-  rewrite of_gmultiset_singleton. iFrame.
 
-  iIntros.
+  iAssert (l ↤{1/4} {[+l'+]} ∗ l ↤{1/4} of_gmultiset (L∖{[+l'+]}))%I with "[Z]" as "(?&?)".
+  { iApply mapsfrom_split. 3,4:done. 1,2:by vm_compute.
+    replace (1 / 2)%Qz with (1/4 + 1/4)%Qz by compute_done.
+    destruct_decide (decide (l' ∈ L)).
+    { rewrite {1}(gmultiset_disj_union_difference' l' L) //.
+      rewrite of_gmultiset_disj_union of_gmultiset_singleton //. }
+    { assert (L = L ∖ {[+l'+]}) as Eq'. multiset_solver.
+      rewrite {1}Eq'. iApply (mapsfrom_weak with "[$]"). by vm_compute.
+      intros. generalize ((L ∖ {[+ l' +]})). intros ?.
+      rewrite smultiset.multiplicity_disj_union. smultiset_solver. } }
+
+  iFrame. iIntros.
   iDestruct (mapsfrom_join with "[$][$]") as "?".
   replace  (1/4 + 1/4)%Qz with (1 / 2)%Qz  by compute_done.
-  rewrite left_id. iExists _. iFrame "Ha".
+  rewrite left_id. iExists _. iFrame "Hz".
   rewrite big_sepS_insert. 2:set_solver.
   iSplitR "Hx".
-  { iRight. iExists _. iFrame. iPureIntro. split_and !.
-    { intros l0. destruct_decide (decide (l0 = l')); subst. split.
-      { intros H'. exfalso. specialize (E3 l'). multiset_solver. }
-      { intros (i',Hi). apply lookup_delete_Some in Hi. destruct Hi as (?&?).
-        exfalso. apply H1; eauto. }
-      split.
-      { intros E. assert (l0 ∈ L) by multiset_solver.
-        apply E2 in H2. destruct H2. exists x. rewrite lookup_delete_ne //.
-        intros  ->. naive_solver. }
-      { intros (i',Hi). apply lookup_delete_Some in Hi. destruct Hi as (?&Hi).
-        assert (l0 ∈ L). apply E2. eauto. multiset_solver. } }
-    { by apply nodup_remove. } }
-  { iApply (update_set_bone with "[$]").
+  { iRight. iExists _. iFrame. iPureIntro.
+    { intros l0.
+      rewrite !multiplicity_difference.
+      specialize (E2 l0). multiset_solver. } }
+  { iApply (update_set_cell with "[$]").
     { intros. eapply stamped_delete; eauto. set_solver. } }
 Qed.
 
-Lemma add_bone h γ M L :
-  (∀ i v, ⌜M !! i = Some (h, v)⌝ -∗ isbone γ h) ∗
-  bones γ M ∗
+Lemma add_cell h γ M L :
+  cells γ M ∗
   h ↤ L =[#]=∗
-  bones γ M ∗ h ↤{1/2} L ∗ isbone γ h.
+  cells γ M ∗ h ↤{1/2} L ∗ iscell γ h.
 Proof.
-  iIntros "(#Hf&[%A (Ha&Hs)]&Hh)". iIntros.
+  iIntros "([%A (Ha&Hs)]&Hh)". iIntros.
   destruct_decide (decide (h ∈ A)).
   { iDestruct (big_sepS_elem_of with "[$]") as "X". done.
     iDestruct "X" as "[? | [% (?&_)]]".
@@ -452,10 +431,6 @@ Proof.
     { iDestruct (mapsfrom_confront with "[$][$]") as "%". by vm_compute.
       congruence. } }
 
-  iAssert (⌜forall i v, M !! i = Some (h,v) -> False⌝)%I as "%".
-  { iIntros (???). iSpecialize ("Hf" with "[%//]").
-    iDestruct (more_cmras.elem_of_gset with "Ha [$]") as "%".
-    congruence. }
   iMod (own_update with "Ha") as "(?&?)".
   { apply auth_update_alloc. apply gset_local_add. }
   rewrite left_id. iFrame. rewrite comm_L. iModIntro.
@@ -465,15 +440,14 @@ Proof.
   iFrame.
   iExists _. iFrame. iApply big_sepS_insert. done. iFrame.
   iRight. iExists ∅. rewrite of_gmultiset_empty. iFrame.
-  iPureIntro. split_and !.
-  { intros l. split; first set_solver. naive_solver. }
-  { rewrite /nodup => ?. rewrite multiplicity_empty. lia. }
+  iPureIntro.
+  { intros l. rewrite multiplicity_empty. lia. }
 Qed.
 
 Lemma schrodinger_kill γ M v l' π  S:
   sizeof l' 2 ∗
   inside π S ∗ schrodinger γ M v l' =[#]=∗
-  inside π (S∪locs v ∪ {[l']}) ∗ †l' ∗ ♢2 ∗ bones γ M.
+  inside π (S ∪ locs v ∪ {[l']}) ∗ †l' ∗ ♢2 ∗ cells γ M.
 Proof.
   iIntros "(?&?&Hcase)". iIntros.
   iMod (dig_debt (S∪locs v∪{[l']}) with "[$][$]") as "(?&?)". set_solver.
@@ -484,14 +458,6 @@ Proof.
     iMod (vmapsfrom_cleanup with "[$][$]") as "(?&?)".
     assert (({[+ l' +]} ⊎ {[-l'-]}) ≡ ∅) as -> by smultiset_solver.
     iSpecialize ("Hback" with "[$]"). by iFrame "#∗". }
-Qed.
-
-Lemma open_phys_stack s p Π γ xs :
-  s ⟸{p} Π ∗ phys_stack γ s xs -∗
-  s ⟸{p} Π ∗ ∃ v, s ↦ [v] ∗ v ↤?{1/2} {[+s+]} ∗ spine γ xs v.
-Proof.
-  iIntros "(?&[?|?])"; last by iFrame.
-  iDestruct (confront_pbt_dag with "[$]") as "%". done.
 Qed.
 
 Ltac clean_debt π :=
@@ -507,7 +473,7 @@ Lemma push_spec (s:loc) (x:val) p q π :
   WITH ⊤
   SOUV {[s]}
   <<< (♢2 ∗ x ⟸?{p} {[π]} ∗ x ↤?{q} ∅) | ∀∀ xs, stack s xs >>>
-  <<< stack s ((x,(p,q))::xs) | (fun r => ⌜r=val_unit⌝)  >>>.
+  <<< stack s ((x,(p,q))::xs) | (fun (_:unit) => True)  >>>.
 Proof.
   iIntros (?) "(HC&H2&H3)". iIntros (Q) "AU".
   iLöb as "IH".
@@ -521,15 +487,14 @@ Proof.
   iIntros "(H5&H3&_)".
   simpl. rewrite left_id.
 
-  iApply @wpc_enter. iIntros (k) "%Ek Hk D".
+  iApply @wpc_enter. iIntros (k) "%Ek HS D".
   apply dom_singleton_inv_L in Ek. destruct Ek as (p'&->).
 
   iApply wp_let_noclean.
   iMod "AU" as (xs0) "(I&[AU _])". solve_atomic.
-  iDestruct "I" as "[%g [%M (#Hmeta&%Hi&I1&I2&I3&I4)]]".
+  iDestruct "I" as "[%g [%M (#Hmeta&I1&I2&I3&I4)]]".
   rewrite -{1}pbt_PBT.
-  iDestruct (open_phys_stack with "[$]") as "(HS&[%h (S1&S2&S3)])".
-  iDestruct (spine_visbone with "S3") as "#T1".
+  iDestruct "I1" as "[%h (S1&S2&S3&#?&S4)]".
 
   iApply wp_tconseq. iApply (tupd_clean_debt h'). iFrame. iIntros "(H7&D)".
   rewrite left_id_L difference_diag_L.
@@ -539,7 +504,7 @@ Proof.
   wp_apply wp_load_inside. compute_done.
   iIntros (?) "(->&_&?&D)".
   iAssert (stack s xs0) with "[-H2 AU H3 D H5 H6 H7 HS]" as "GO".
-  { iExists g,M. iFrame "#%∗". iRight. iExists _. iFrame. }
+  { iSmash. }
   iMod ("AU" with "GO") as "AU". iModIntro.
   clear dependent xs0 M.
 
@@ -547,42 +512,40 @@ Proof.
 
   iApply wp_let_noclean.
   iMod "AU" as (xs0) "(I&[AU _])". solve_atomic.
-  iDestruct (open_stack_inv_meta with "Hmeta I") as "[%M (%&I1&I2&I3&I4)]".
+  iDestruct (open_stack_inv_meta with "Hmeta I") as "[%M (I1&I2&I3&I4)]".
   rewrite difference_diag_L.
   iMod (register h' with "[$][$][$][$][$]") as
-    "[%i [%M' (%&?&?&Hreg&Hcase)]]".
-  done.
+    "[%M' (?&?&Hreg&Hcase)]".
 
   iDestruct "Hcase" as "[ (dag&?) | (Hmf&Hback)]".
   (* h was reclaimed by a concurrent [pop] *)
   { iDestruct "dag" as "[%l (->&#?)]".
 
-    iApply wp_tconseq. iApply unreg. done. iFrame "∗#".
-    iIntros "[%M'' (%&R1&R2&Hcase)]".
+    iApply wp_tconseq. iApply (unreg _ _ _ _ M'). iFrame "∗#".
+    iIntros "[%M'' (R1&R2&Hcase)]".
     iApply wp_tconseq. iApply schrodinger_kill. iFrame "∗#".
     iIntros "(D&#?&R3&?)".
 
     wp_apply wp_store_dead. compute_done.
     iIntros (?) "(->&_&_)".
     iMod ("AU" with "[-H2 H3 D HS R3]") as "AU".
-    { iExists _,_. iFrame "#∗". eauto. }
+    { iSmash. }
     iIntros "!> _".
     clear dependent xs0 M M' M''.
 
     iApply wp_let_noclean.
     iMod "AU" as (xs0) "(I&[AU _])". solve_atomic.
-    iDestruct (open_stack_inv_meta with "Hmeta I") as "[%M (%&I1&I2&I3&I4)]".
-
-    iDestruct (open_phys_stack with "[$]") as "(HS&[%h (S1&S2&S3)])".
+    iDestruct (open_stack_inv_meta with "Hmeta I") as "[%M (I1&I2&I3&I4)]".
+    iDestruct "I1" as "[%h (S1&S2&S3&S4&S5)]".
     destruct_decide (decide (h=l)).
     { subst. iApply wp_tconseq. simpl.
       iApply (confront_mapsfrom_dag _ l). 2:iFrame. compute_done.
-      iFrame "#". iIntros. done. }
+      iSteps. }
 
     wp_apply wp_cas_fail. 1-3:done.
     iIntros (?) "(->&_&?)".
     iMod ("AU" with "[-H2 H3 D HS R3]") as "AU".
-    { iExists _,_. iFrame "#∗%". iRight. iExists _. by iFrame. }
+    { iSmash. }
 
     iIntros "!> _". simpl. iApply wp_if. iIntros "!> _".
     iApply wp_tconseq. iApply (vmapsfrom_cleanup x h'). iFrame "#∗". iIntros.
@@ -593,35 +556,35 @@ Proof.
     rewrite union_idemp_L.
 
     clean_debt π.
-    iApply wpc_exit; last iFrame. set_solver. rewrite dom_singleton_L.
+    iApply @wpc_exit; last iFrame. set_solver. rewrite dom_singleton_L.
     rewrite -pbt_PBT. iFrame.
     iApply ("IH" with "[$][$][$][$]"). }
 
   (* h is still allocated, we proceed. *)
-  wp_apply wp_store. intros. compute_done. compute_done.
+  wp_apply wp_store. intros. 1,2:compute_done.
 
   iIntros (?) "(->&_&H5&X&_)".
   rewrite left_id.
   iSpecialize ("Hback" with "[$]").
   iMod ("AU" with "[-H2 H3 H5 Hreg D HS]") as "AU".
-  { iExists _,M'. iFrame "#%∗". }
+  { iSmash. }
 
   clear dependent xs0 M M'.
   iIntros "!> _". simpl.
 
   iApply wp_let_noclean.
   iMod "AU" as (xs0) "(I&AU)". solve_atomic.
-  iDestruct (open_stack_inv_meta with "Hmeta I") as "[%M (%&I1&I2&I3&I4)]".
-  iDestruct (open_phys_stack with "[$]") as "(HS&[%h0 (S1&S2&S3)])".
+  iDestruct (open_stack_inv_meta with "Hmeta I") as "[%M (I1&I2&I3&I4)]".
+  iDestruct "I1" as "[%h0 (S1&S2&S3&S4&S5)]".
 
-  iApply wp_tconseq. iApply unreg. done. iFrame "#∗".
-  iIntros "[%M' (%&R1&R2&Hcase)]".
+  iApply wp_tconseq. iApply (unreg _ _ _ _ M). iFrame "#∗".
+  iIntros "[%M' (R1&R2&Hcase)]".
 
   destruct_decide (decide (h=h0)); try subst h0.
   (* CAS will succeed. *)
   { iDestruct "Hcase" as "[ ([% (->&?)]&_) | (X1&X2&X3&Hback)]".
     { iApply wp_tconseq. iApply confront_mapsfrom_dag.
-      2:iFrame. compute_done. iIntros "?". done. }
+      2:iFrame. compute_done. iSteps. }
 
     iApply wp_tconseq. iApply (tupd_vclean_debt x). iFrame. iIntros "(?&D)".
     rewrite difference_diag_L.
@@ -639,23 +602,16 @@ Proof.
     iDestruct (vmapsfrom_split with "[$]") as "(?&?)". 1,2:by vm_compute.
     iSpecialize ("Hback" with "[$]").
 
-    iAssert (∀ i v, ⌜M' !! i = Some (h', v)⌝ -∗ isbone (gb g) h')%I as "#Hok".
-    { iIntros (?? Hi). simpl.
-      iDestruct (big_sepM_lookup with "R2") as "(?&_)".
-      apply Hi. done. }
-
-    iApply wp_tconseq. iApply add_bone. iFrame "#∗". iIntros "(?&Hh&#?)".
+    iApply wp_tconseq. iApply add_cell. iFrame "#∗". iIntros "(?&Hh&#?)".
     iApply wp_val.
 
     iDestruct "AU" as "[_ AU]".
     iMod ("AU" with "[-D HS]") as "HPOST".
-    { iExists _,_. iFrame "%∗ Hmeta".
-      iRight. iExists _. iFrame. simpl. iFrame.
-      iExists h',h. iFrame "∗#". eauto. }
+    { iSmash. }
 
     iIntros "!> _". iApply wp_if. iModIntro. iIntros "_".
     clean_debt π.
-    iApply wpc_exit; last iFrame. set_solver. rewrite pbt_PBT. iFrame.
+    iApply @wpc_exit; last iFrame. set_solver. rewrite pbt_PBT. iFrame.
     do 2 iStep. iApply "HPOST". by iFrame. }
   (* Reboot *)
   { iApply wp_tconseq. iApply schrodinger_kill. iFrame "#∗".
@@ -669,36 +625,37 @@ Proof.
 
     iDestruct "AU" as "[AU _]".
     iMod ("AU" with "[-R3 H2 D cred HS]") as "AU".
-    { iExists _,_. iFrame "Hmeta %∗". iRight. iExists _. iFrame. }
+    { iSmash. }
     iIntros "!> _". simpl. iApply wp_if. iModIntro. iIntros "_".
 
     iApply wp_tconseq. iApply (debt_vtransfer x). iFrame. iIntros "(?&?)".
     iApply wp_tconseq. iApply (debt_vtransfer s). iFrame. iIntros "(?&?)".
     rewrite union_idemp_L.
     clean_debt π.
-    iApply wpc_exit; last iFrame. set_solver. rewrite dom_singleton_L -pbt_PBT. iFrame.
-    iApply ("IH" with "[$][$][$][$]"). }
+    iApply @wpc_exit; last iFrame. set_solver. rewrite dom_singleton_L -pbt_PBT.
+    iFrame. iApply ("IH" with "[$][$][$][$]"). }
+  Unshelve. exact inhabitant.
 Qed.
 
 Lemma free_protected (l:loc) γ L M :
-  nodup L ->
-  (forall (l':loc), l' ∈ L -> ∃ π, M !! π = Some (l, l')) ->
-  protection γ M ∗
+  stamped l L M ->
+  outsiders γ M ∗
   l ↤ of_gmultiset L =[#]=∗
-  (l ↤ ∅ ∗ (†l -∗ protection γ M)).
+  (l ↤ ∅ ∗ (†l -∗ outsiders γ M)).
 Proof.
-  iIntros (E2 E3) "(Hp&?)". iIntros.
-  iInduction L as [|l' L] "IH" using gmultiset_ind forall (M E2 E3).
+  iIntros (E) "(Hp&?)". iIntros.
+  iInduction L as [|l' L] "IH" using gmultiset_ind forall (M E).
   { rewrite of_gmultiset_empty.
     iFrame. iModIntro. eauto. }
 
   rewrite of_gmultiset_disj_union of_gmultiset_singleton.
-  assert (∃ (π:thread_id), M !! π = Some (l, l')) as (i,Hi).
-  { apply E3. multiset_solver. }
+  assert ((l, l') ∈ M) as Hi.
+  { specialize (E l'). rewrite multiplicity_disj_union in E.
+    multiset_solver. }
 
-  rewrite {3}/protection. rewrite big_sepM_delete //. simpl.
+  rewrite {3}/outsiders. rewrite big_sepMS_delete //. simpl.
   iDestruct "Hp" as "(X&Hp)".
-  iDestruct "X" as "(#?&#?&[(?&?)|(?&_)])"; last first.
+  iDestruct "X" as "[(?&?&?)|(?&_)]"; last first.
   { iMod (confront_mapsfrom_dag with "[$][$]") as "(_&?)"; last done.
     by vm_compute. }
 
@@ -706,25 +663,23 @@ Proof.
   iMod (mapsfrom_cleanup with "[$][$]") as "(?&?)".
   assert (({[+ l' +]} ⊎ of_gmultiset L ⊎ {[-l'-]}) ≡ of_gmultiset L) as -> by smultiset_solver.
 
-  iMod ("IH" with "[%][%][$][$][$]") as "(?&?&Hb)".
-  { intros l0. specialize (E2 l0). rewrite multiplicity_disj_union in E2. multiset_solver. }
-  { intros l0 E. destruct (E3 l0). multiset_solver.
-    exists x. rewrite lookup_delete_ne //. intros ->.
-    rewrite Hi in H0. inversion H0. subst. specialize (E2 l0).
-    rewrite multiplicity_disj_union in E2. multiset_solver. }
+  iMod ("IH" $! (M ∖ {[+ (l, l') +]}) with "[%][$][$][$]") as "(?&?&Hb)".
+  { intros l0. specialize (E l0). rewrite multiplicity_disj_union in E.
+    rewrite multiplicity_difference.
+    multiset_solver. }
 
   iFrame. iModIntro. iIntros.
-  iSpecialize ("Hb" with "[$]"). iApply big_sepM_delete. done.
+  iSpecialize ("Hb" with "[$]"). iApply big_sepMS_delete. done.
   iFrame. simpl. iFrame "#∗".
 Qed.
 
-Lemma free_bone γ l M :
+Lemma free_cell γ l M :
   sizeof l 2 ∗
-  isbone γ l ∗
+  iscell γ l ∗
   l ⟸ ∅ ∗ l ↤{1/2} ∅ ∗
-  protection γ M ∗
-  bones γ M =[#]=∗
-  †l ∗ ♢2 ∗ protection γ M ∗ bones γ M.
+  outsiders γ M ∗
+  cells γ M =[#]=∗
+  †l ∗ ♢2 ∗ outsiders γ M ∗ cells γ M.
 Proof.
   iIntros "(?&?&?&Hp&Hl&[% (Ha&X)])". iIntros.
   iDestruct (more_cmras.elem_of_gset with "Ha [$]") as "%Hv".
@@ -732,13 +687,12 @@ Proof.
   2:{ rewrite union_comm_L difference_union_L. set_solver. }
   rewrite big_sepS_insert. 2:set_solver.
 
-  iDestruct "X" as "([?|[% (?&%E2&%E3)]]&?)".
+  iDestruct "X" as "([?|[% (?&%E)]]&?)".
   { iMod (confront_mapsfrom_dag with "[$][$]") as "(_&?)"; last done. by vm_compute. }
   iDestruct (mapsfrom_join with "[$][$]") as "?". rewrite Qz_div_2 right_id.
 
-  iMod (free_protected with "[$][$]") as "(?&?&Hb)".
+  iMod (free_protected _ _ _ M with "[$][$]") as "(?&?&Hb)".
   { done. }
-  { intros. by eapply E2. }
   iMod (interp_free'' with "[$][$]") as "(?&?&#?)".
   iSpecialize ("Hb" with "[$]"). iFrame "#∗". iModIntro. iExists _. iFrame "Ha".
   iApply big_sepS_insert. set_solver. iFrame. by iLeft.
@@ -757,32 +711,26 @@ Proof.
 
   wpc_call.
 
-  iApply @wpc_enter. iIntros (k) "%Ek Hk D".
+  iApply @wpc_enter. iIntros (k) "%Ek HS D".
   apply dom_singleton_inv_L in Ek. destruct Ek as (p'&->).
 
   iApply wp_let_noclean.
   iMod "AU" as (xs0) "(I&[AU _])". solve_atomic.
-  iDestruct "I" as "[%g [%M (#Hmeta&%Hi&I1&I2&I3&I4)]]".
+  iDestruct "I" as "[%g [%M (#Hmeta&I1&I2&I3&I4)]]".
   rewrite -{1}pbt_PBT.
-  iDestruct (open_phys_stack with "[$]") as "(HS&[%h (S1&S2&S3)])".
-
-  (* LATER copy/pasted *)
-  iAssert (visbone g.(gb) h) as "#T1".
-  { destruct xs0 as [|(?&?&?)]. iDestruct "S3" as "->". by iLeft.
-    iDestruct "S3" as "[%[% (->&?&?&?&?)]]". iRight. iExists _.
-    by iFrame. }
+  iDestruct "I1" as "[%h (S1&S2&S3&#?&S5)]".
 
   wp_apply wp_load_inside. compute_done.
   iIntros (?) "(->&_&?&D)".
 
-  iAssert (⌜h=val_unit⌝ ∨ ∃ l x h', ⌜h=val_loc l⌝ ∗ l ↦□ [x;h'] ∗ visbone _ h')%I as "#Hcase".
+  iAssert (⌜h=val_unit⌝ ∨ ∃ l x h', ⌜h=val_loc l⌝ ∗ l ↦□ [x;h'] ∗ reg _ h')%I as "#Hcase".
   { destruct xs0 as [|(?&?&?)].
-    { iDestruct "S3" as "->". eauto. }
-    { iDestruct "S3" as "[%[% (->&?&?&?&?&?&?&?)]]". iRight. iExists _,_,_.
-      iDestruct (spine_visbone with "[$]") as "?". by iFrame. } }
+    { iDestruct "S5" as "->". eauto. }
+    { iDestruct "S5" as "[%[% (->&?&?&?&?&?&?)]]". iRight. iExists _,_,_.
+      by iFrame. } }
 
   iMod ("AU" with "[-D HS]") as "AU".
-  { iExists _,_. iFrame "Hmeta ∗%". iRight. iExists _. iFrame. }
+  { iSmash. }
   iIntros "!> _". simpl.
   clear dependent xs0 M.
 
@@ -806,8 +754,8 @@ Proof.
   iApply wp_let_noclean.
 
   iMod "AU" as (xs0) "(I&AU)". solve_atomic.
-  iDestruct (open_stack_inv_meta with "Hmeta I") as "[%M (%Hi&I1&I2&I3&I4)]".
-  iDestruct (open_phys_stack with "[$]") as "(HS&[%h0 (S1&S2&S3)])".
+  iDestruct (open_stack_inv_meta with "Hmeta I") as "[%M (I1&I2&I3&I4)]".
+  iDestruct "I1" as "[%h0 (S1&S2&S3&S4&S5)]".
 
   destruct_decide (decide (h0=l)).
   { subst.
@@ -815,8 +763,8 @@ Proof.
     iDestruct "AU" as "[_ AU]". rename xs0 into xs.
 
     destruct xs as [|(v,(p,q)) xs].
-    { iDestruct "S3" as "%". congruence. }
-    iDestruct "S3" as "[%[% (%Eq&?&?&Hv&R1&R2&R3&?)]]". inversion Eq. subst l0. clear Eq.
+    { iDestruct "S5" as "%". congruence. }
+    iDestruct "S5" as "[%[% (%Eq&?&?&Hv&R1&R2&R3&?)]]". inversion Eq. subst l0. clear Eq.
     iDestruct (mapsto_agree with "[$][$]") as "%Eq". inversion Eq. subst v v'. simpl. clear Eq.
 
     assert ((1/2)%Qz = (1/4 + 1/4)%Qz)%Qz as Eq by compute_done.
@@ -833,7 +781,8 @@ Proof.
     rewrite Qz_add_0_l.
 
     iDestruct (mapsto_extract_size l with "[$]") as "?". simpl.
-    iApply wp_tconseq. iApply free_bone. iFrame.
+    iDestruct "S4" as "[%|[%l0 (%Eq'&?)]]". congruence. inversion Eq'. subst l0.
+    iApply wp_tconseq. iApply (free_cell _ _ M). iFrame.
     iIntros "(#?&cred&?)".
 
     iDestruct (vmapsfrom_join with "[$]") as "?". rewrite -Eq.
@@ -872,41 +821,43 @@ Proof.
     iApply ("IH" with "[$]"). }
 Qed.
 
-Lemma free_spine γ l xs M :
-  spine γ xs l ∗ l ↤?{1/2} ∅ ∗
-  protection γ M ∗
-  bones γ M =[#]=∗
-  ♢(2*length xs) ∗ protection γ M ∗ bones γ M ∗
+Lemma free_innerList γ l xs M :
+  innerList γ xs l ∗
+  l ⟸? ∅ ∗ reg γ l ∗ l ↤?{1/2} ∅ ∗
+  outsiders γ M ∗
+  cells γ M =[#]=∗
+  ♢(2*length xs) ∗ outsiders γ M ∗ cells γ M ∗
   handles xs.
 Proof.
-  iIntros "(Hs&?&?&?)". iIntros.
+  iIntros "(Hs&?&His&?&?)". iIntros.
 
   iInduction xs as [|(x,(p,q)) xs] "IH" forall (l).
   { simpl. rewrite right_absorb.
     iMod diamonds_zero. rewrite handles_nil. iSmash. }
   iDestruct "Hs" as "[%[% (->&?&?&?&?&?&?&?)]]".
   iDestruct (mapsto_extract_size with "[$]") as "?".
-  iMod (free_bone with "[$][$]") as "(?&#?&?&?&?)".
+  iDestruct "His" as "[% | [%l' (%Eq'&?)]]". congruence. inversion Eq'. subst l'.
+  iMod (free_cell _ _ M with "[$][$]") as "(?&#?&?&?&?)".
   iMod (vmapsfrom_cleanup x with "[$][$]") as "(?&?)".
   iMod (vmapsfrom_cleanup v' with "[$][$]") as "(?&?)".
   assert (({[+ l0 +]} ⊎ {[-l0-]}) ≡ ∅) as -> by smultiset_solver.
-  iMod ("IH" with "[$][$][$][$][$]") as "(?&?&?&?&?)".
+  iMod ("IH" with "[$][$][$][$][$][$]") as "(?&?&?&?&?)".
   iFrame. iModIntro. simpl.
   conclude_diamonds.
 Qed.
 
 Lemma treiber_free s xs :
   stack s xs ∗ s ↤ ∅ ∗ s ⟸ ∅ =[#]=∗
-  ♢(1 + 2*length xs) ∗ handles xs.
+  †s ∗ ♢(1 + 2*length xs) ∗ handles xs.
 Proof.
   iIntros "(I&?&?)". iIntros.
-  iDestruct "I" as "[%g [%M (_&%Hi&I1&I2&I3&I4)]]".
-  iDestruct (open_phys_stack with "[$]") as "(HS&[%h0 (S1&S2&S3)])".
+  iDestruct "I" as "[%g [%M (_&I1&I2&I3&I4)]]".
+  iDestruct "I1" as "[%h0 (S1&S2&S3&S4&S5)]".
   iMod (interp_free' s with "[$][$]") as "(?&C1&?&#?)".
   iMod (vmapsfrom_cleanup with "[$][$]") as "(?&?)".
 
   assert (({[+ s +]} ⊎ {[-s-]}) ≡ ∅) as -> by smultiset_solver.
-  iMod (free_spine with "[$][$]") as "(?&C2&?&?&?)". iFrame.
+  iMod (free_innerList _ _ _ M with "[$][$]") as "(?&C2&?&?&?)". iFrame "#∗".
   conclude_diamonds.
 Qed.
 
