src/examples/sequential/stack/stack.v
@@ -1,4 +1,4 @@
-From irisfit.examples Require Import proofmode.
+From irisfit.examples Require Import proofmode treiber.
 From irisfit.examples.sequential Require Import list.
 
 (* This file introduces possibly bounded stacks and their specifications. *)
@@ -7,6 +7,15 @@ Definition size_lt n (c:option positive) :=
   match c with
   | Some c => n < Pos.to_nat c
   | None => True end.
+
+(* Coq has trouble inferring things if I use an separated interp, and a separated
+   "extended ghost state". So I bundle the two. *)
+Class interpGSMore (Σ:gFunctors) : Set :=
+  { mi1 : interpGS0 Σ;
+    mi2 : stackG Σ
+  }.
+
+Global Existing Instances mi1 mi2.
 
 Module Type StackOf.
   Parameter capacity : option positive.
@@ -23,37 +32,37 @@ Module Type StackOf.
   Axiom locs_stack_is_empty : locs stack_is_empty = ∅.
   Axiom locs_stack_is_full : locs stack_is_full = ∅.
 
-  Parameter StackOf : forall `{interpGS0 Σ} {A} (R:A -> val -> iProp Σ),
-      list (A * (Qz * Qp)) -> loc -> iProp Σ.
+  Parameter StackOf : forall `{interpGSMore Σ} {A} (R:A -> val -> iProp Σ),
+      list (A * (Qp * Qz)) -> loc -> iProp Σ.
 
   Parameter empty_cost : Qz.
   Parameter cell_cost : Qz.
 
-  Axiom stack_empty_spec : forall `{interpGS0 Σ} π A (R:A -> val -> iProp Σ),
+  Axiom stack_empty_spec : forall `{interpGSMore Σ} π A (R:A -> val -> iProp Σ),
       CODE (stack_empty [[]])
       TID π
       PRE  (♢ empty_cost)
       POST (fun s => StackOf R [] s ∗ s ⟸ {[π]} ∗ s ↤ ∅).
 
-  Axiom stack_push_spec : forall `{interpGS0 Σ} π A (R:A -> val -> iProp Σ),
+  Axiom stack_push_spec : forall `{interpGSMore Σ} π A (R:A -> val -> iProp Σ),
     forall s qp qz v x xs,
       size_lt (length xs) capacity ->
       qz ≠ 0%Qz ->
-      CODE (stack_push [[v, s]])
+      CODE (stack_push [[s, v]])
       TID π
       SOUV {[s]}
       PRE  (♢ cell_cost ∗ StackOf R xs s ∗ R x v ∗ v ⟸?{qp} {[π]} ∗ v ↤?{qz} ∅)
-      POST (fun (_:unit) => StackOf R ((x,(qz,qp))::xs) s).
+      POST (fun (_:unit) => StackOf R ((x,(qp,qz))::xs) s).
 
-  Axiom stack_pop_spec : forall `{interpGS0 Σ} π A (R:A -> val -> iProp Σ),
+  Axiom stack_pop_spec : forall `{interpGSMore Σ} π A (R:A -> val -> iProp Σ),
     forall s qp qz x xs,
       CODE (stack_pop [[s]])
       TID π
       SOUV {[s]}
-      PRE  (StackOf R ((x,(qz,qp))::xs) s)
+      PRE  (StackOf R ((x,(qp,qz))::xs) s)
       POST (fun v => R x v ∗ v ⟸?{qp} {[π]} ∗ v ↤?{qz} ∅ ∗ StackOf R xs s ∗ ♢ cell_cost).
 
-  Axiom stack_is_empty_spec : forall `{interpGS0 Σ} π A (R:A -> val -> iProp Σ),
+  Axiom stack_is_empty_spec : forall `{interpGSMore Σ} π A (R:A -> val -> iProp Σ),
     forall xs s,
       CODE (stack_is_empty [[s]])
       TID π
@@ -61,7 +70,7 @@ Module Type StackOf.
       PRE  (StackOf R xs s)
       POST (fun (b:bool) => ⌜b <-> xs=nil⌝ ∗ StackOf R xs s).
 
-  Axiom stack_is_full_spec : forall `{interpGS0 Σ} π A (R:A -> val -> iProp Σ),
+  Axiom stack_is_full_spec : forall `{interpGSMore Σ} π A (R:A -> val -> iProp Σ),
     forall xs s,
       CODE (stack_is_full [[s]])
       TID π
@@ -69,7 +78,7 @@ Module Type StackOf.
       PRE (StackOf R xs s)
       POST (fun (b:bool) => ⌜b <-> ¬ (size_lt (length xs) capacity)⌝ ∗ StackOf R xs s).
 
-  Axiom stack_free : forall `{interpGS0 Σ} A (R:A -> val -> iProp Σ),
+  Axiom stack_free : forall `{interpGSMore Σ} A (R:A -> val -> iProp Σ),
     forall s xs,
       s ⟸ ∅ ∗ s ↤ ∅ ∗ StackOf R xs s =[#]=∗
       ♢(empty_cost + cell_cost*length xs) ∗ † s ∗
@@ -78,33 +87,32 @@ End StackOf.
 
 Module Type Capacity.
   Parameter capacity : positive.
-
 End Capacity.
 
 Module MoreStackOf(St:StackOf).
 Export St.
 
-Lemma stack_pop_spec' `{interpGS0 Σ} π A (R:A -> val -> iProp Σ) xs s:
+Lemma stack_pop_spec' `{interpGSMore Σ} π A (R:A -> val -> iProp Σ) xs s:
   xs ≠ nil ->
   CODE (stack_pop [[s]])
   TID π
   SOUV {[s]}
   PRE (StackOf R xs s)
-  POST (fun v => ∃ x xs' qz qp, ⌜xs=(x,(qz,qp))::xs'⌝ ∗ R x v ∗ v ⟸?{qp} {[π]} ∗ v ↤?{qz} ∅ ∗ StackOf R xs' s ∗ ♢ cell_cost).
+  POST (fun v => ∃ x xs' qz qp, ⌜xs=(x,(qp,qz))::xs'⌝ ∗ R x v ∗ v ⟸?{qp} {[π]} ∗ v ↤?{qz} ∅ ∗ StackOf R xs' s ∗ ♢ cell_cost).
 Proof.
-  iIntros. destruct xs as [|(x,(qz,qp)) xs']; try easy.
+  iIntros. destruct xs as [|(x,(qp,qz)) xs']; try easy.
   iApply (wpc_mono with "[-]").
-  { iApply stack_pop_spec. iFrame. }
+  { iApply stack_pop_spec. done. }
   iIntros (?) "(?&?&?&?&?)".
   iExists _,_,_,_. iFrame. eauto.
 Qed.
 
 (* A stack free for empty stacks *)
-Lemma empty_stack_free `{interpGS0 Σ} A (R:A -> val -> iProp Σ) s :
+Lemma empty_stack_free `{interpGSMore Σ} A (R:A -> val -> iProp Σ) s :
   s ⟸ ∅ ∗ s ↤ ∅ ∗ StackOf R nil s =[#]=∗ ♢ empty_cost.
 Proof.
   iIntros "(?&?)". iIntros.
-  iMod (stack_free with "[$] [$]") as "(?&?&?)".
+  iMod (@stack_free with "[$] [$]") as "(?&?&?)".
   iFrame.
   simpl. rewrite right_absorb right_id.
   by iFrame.
@@ -116,11 +124,11 @@ End MoreStackOf.
 Module StackDominant(St:StackOf).
 Export St.
 
-Definition StackDominantOf `{!interpGS0 Σ} {A} (R:A -> val -> iProp Σ)
+Definition StackDominantOf `{interpGSMore Σ} {A} (R:A -> val -> iProp Σ)
   qp (xs:list A) (s:loc) : iProp Σ :=
-  StackOf R (fmap (fun v => (v,(1%Qz,qp))) xs) s.
+  StackOf R (fmap (fun v => (v,(qp,1%Qz))) xs) s.
 
-Lemma stack_is_empty_spec_dominant `{interpGS0 Σ} π A (R:A -> val -> iProp Σ) qp xs s :
+Lemma stack_is_empty_spec_dominant `{interpGSMore Σ} π A (R:A -> val -> iProp Σ) qp xs s :
   CODE (stack_is_empty [[s]])
   TID π
   SOUV {[s]}
@@ -134,7 +142,7 @@ Proof.
   now destruct xs.
 Qed.
 
-Lemma stack_is_full_spec_dominant `{interpGS0 Σ} π A (R:A -> val -> iProp Σ) qp xs s :
+Lemma stack_is_full_spec_dominant `{interpGSMore Σ} π A (R:A -> val -> iProp Σ) qp xs s :
   CODE (stack_is_full [[s]])
   TID π
   SOUV {[s]}
@@ -147,7 +155,7 @@ Proof.
   rewrite fmap_length. eauto.
 Qed.
 
-Lemma stack_empty_dominant_spec `{!interpGS0 Σ} π A (R:A -> val -> iProp Σ) qp :
+Lemma stack_empty_dominant_spec `{interpGSMore Σ} π A (R:A -> val -> iProp Σ) qp :
   CODE (stack_empty [[]])
   TID π
   PRE (♢ empty_cost)
@@ -158,13 +166,13 @@ Proof.
   iIntros. iFrame.
 Qed.
 
-Lemma stack_push_dominant_spec `{!interpGS0 Σ} π A (R:A -> val -> iProp Σ) qp x v xs s :
+Lemma stack_push_dominant_spec `{interpGSMore Σ} π A (R:A -> val -> iProp Σ) qp x v xs s :
   size_lt (length xs) capacity ->
-  CODE (stack_push [[v, s]])
+  CODE (stack_push [[s, v]])
   TID π
   SOUV {[s]}
   PRE (♢ cell_cost ∗ StackDominantOf R qp xs s ∗ v ↤? ∅ ∗ v ⟸?{qp} {[π]} ∗ R x v)
-  POST (fun tt => StackDominantOf R qp (x::xs) s).
+  POST (fun (_:unit) => StackDominantOf R qp (x::xs) s).
 Proof.
   iIntros (?) "(? & ? & ? & ? & ?)".
   wpc_apply @stack_push_spec.
@@ -173,7 +181,7 @@ Proof.
   iFrame. iIntros. iFrame.
 Qed.
 
-Lemma stack_pop_dominant_spec `{!interpGS0 Σ} π A (R:A -> val -> iProp Σ) qp x xs s :
+Lemma stack_pop_dominant_spec `{interpGSMore Σ} π A (R:A -> val -> iProp Σ) qp x xs s :
   CODE (stack_pop [[s]])
   TID π
   SOUV {[s]}
@@ -185,7 +193,7 @@ Proof.
   iFrame.
 Qed.
 
-Lemma stack_pop_dominant_spec' `{!interpGS0 Σ} π A (R:A -> val -> iProp Σ) qp xs s :
+Lemma stack_pop_dominant_spec' `{interpGSMore Σ} π A (R:A -> val -> iProp Σ) qp xs s :
   xs ≠ nil ->
   CODE (stack_pop [[s]])
   TID π
@@ -194,18 +202,18 @@ Lemma stack_pop_dominant_spec' `{!interpGS0 Σ} π A (R:A -> val -> iProp Σ) qp
   POST (fun v => ∃ y ys, ⌜xs=y::ys⌝ ∗ R y v ∗ v ↤? ∅ ∗ v ⟸?{qp} {[π]} ∗ StackDominantOf R qp ys s ∗ ♢ cell_cost).
 Proof.
   iIntros (?) "?".
-  destruct xs as [|v tl]; try easy.
-  wpc_apply @stack_pop_dominant_spec. eauto.
+  destruct xs as [|v tl]; try done.
+  wpc_apply @stack_pop_dominant_spec; eauto.
 Qed.
 
-Lemma stack_dominant_free `{!interpGS0 Σ} A (R:A -> val -> iProp Σ) qp (xs:list A) s :
+Lemma stack_dominant_free `{interpGSMore Σ} A (R:A -> val -> iProp Σ) qp (xs:list A) s :
   s ⟸ ∅ ∗ s ↤ ∅ ∗ StackDominantOf R qp xs s =[#]=∗
   ♢(empty_cost+cell_cost*length xs) ∗ †s ∗
   (∃ vs, [∗ list] x;v ∈ xs; vs,
      v ↤? ∅ ∗ v ⟸?{qp} ∅ ∗ R x v).
 Proof.
   iIntros "(Hk & Hs1 & Hs2)". iIntros.
-  iMod (stack_free _ R s (((λ v, (v, (1%Qz,qp))) <$> xs)) with "[$] [$]") as "(? & ? & ? & [%vs Hvs])".
+  iMod (stack_free _ R s (((λ v, (v, (qp,1%Qz))) <$> xs)) with "[$] [$]") as "(? & ? & ? & [%vs Hvs])".
   iModIntro. iFrame. rewrite fmap_length. iFrame.
   iExists vs.
 
@@ -221,7 +229,7 @@ End StackDominant.
 Module PaperStack(S:StackOf).
 Import S.
 
-Definition dupf : val * Qp -> val * (Qz * Qp) := fun '(v,q) => (v,(q:Qz,q)).
+Definition dupf : val * Qp -> val * (Qp * Qz) := fun '(v,q) => (v,(q,q:Qz)).
 
 Lemma soup_mixer `{interpGS0 Σ} (xs:list (val*Qp)) vs :
   soup (λ x y : val, ⌜x = y⌝) ∅ (dupf <$> xs) vs -∗
@@ -235,31 +243,31 @@ Proof.
   iFrame. iApply "IH". iFrame.
 Qed.
 
-Definition Stack `{interpGS0 Σ} (L:list (val * Qp)) (l:loc) : iProp Σ :=
+Definition Stack `{interpGSMore Σ} (L:list (val * Qp)) (l:loc) : iProp Σ :=
   @StackOf _ _ val (fun (x y:val) => ⌜x = y⌝)%I (dupf <$> L) l.
 
-Lemma stack_empty_spec `{interpGS0 Σ} π :
+Lemma stack_empty_spec `{interpGSMore Σ} π :
   CODE (stack_empty [[]])
   TID π
   PRE  (♢ empty_cost)
   POST (fun s => Stack [] s ∗ s ⟸ {[π]} ∗ s ↤ ∅).
-Proof. apply stack_empty_spec. Qed.
+Proof. eauto using stack_empty_spec. Qed.
 
-Lemma stack_push_spec `{interpGS0 Σ} π s qp x xs :
+Lemma stack_push_spec `{interpGSMore Σ} π s qp x xs :
   size_lt (length xs) capacity ->
-  CODE (stack_push [[x, s]])
+  CODE (stack_push [[s,x]])
   TID π
   SOUV {[s]}
   PRE  (♢ cell_cost ∗ Stack xs s ∗ x ⟸?{qp} {[π]} ∗ x ↤?{qp} ∅)
-  POST (fun tt => Stack ((x,qp)::xs) s).
+  POST (fun (_:unit) => Stack ((x,qp)::xs) s).
 Proof.
   iIntros (?) "(? & ? & ? & ?)".
-  wpc_apply stack_push_spec; eauto.
+  wpc_apply @stack_push_spec; eauto.
   { rewrite fmap_length //. }
   { apply Qp_to_Qz_ne_zero. }
 Qed.
 
-Lemma stack_pop_spec `{interpGS0 Σ} π s qp x xs :
+Lemma stack_pop_spec `{interpGSMore Σ} π s qp x xs :
   CODE (stack_pop [[s]])
   TID π
   SOUV {[s]}
@@ -267,11 +275,11 @@ Lemma stack_pop_spec `{interpGS0 Σ} π s qp x xs :
   POST (fun v => x ⟸?{qp} {[π]} ∗ v ↤?{qp} ∅ ∗ Stack xs s ∗ ♢ cell_cost).
 Proof.
   iIntros.
-  wpc_apply stack_pop_spec. eauto. iIntros (?) "(% & ? & ? & ?)".
+  wpc_apply stack_pop_spec; eauto. iIntros (?) "(% & ? & ? & ?)".
   subst. iFrame.
 Qed.
 
-Lemma stack_is_empty_spec `{interpGS0 Σ} π xs s :
+Lemma stack_is_empty_spec `{interpGSMore Σ} π xs s :
   CODE (stack_is_empty [[s]])
   TID π
   SOUV {[s]}
@@ -279,12 +287,12 @@ Lemma stack_is_empty_spec `{interpGS0 Σ} π xs s :
   POST (fun (b:bool) => ⌜b <-> xs=nil⌝ ∗ Stack xs s).
 Proof.
   iIntros.
-  wpc_apply stack_is_empty_spec. eauto. iIntros (?) "(% & ?)".
+  wpc_apply stack_is_empty_spec; eauto. iIntros (?) "(% & ?)".
   iFrame.
   iPureIntro. destruct xs; simpl in *; naive_solver.
 Qed.
 
-Lemma stack_is_full_spec `{interpGS0 Σ} π xs s :
+Lemma stack_is_full_spec `{interpGSMore Σ} π xs s :
   CODE (stack_is_full [[s]])
   TID π
   SOUV {[s]}
@@ -297,13 +305,13 @@ Proof.
   eauto.
 Qed.
 
-Lemma stack_free `{interpGS0 Σ} (xs:list (val*Qp)) s :
+Lemma stack_free `{interpGSMore Σ} (xs:list (val*Qp)) s :
   s ⟸ ∅ ∗ s ↤ ∅ ∗ Stack xs s =[#]=∗
     ♢(empty_cost + cell_cost*length xs) ∗ † s ∗
     ([∗ list] x ∈ xs, (x.1 ↤?{x.2:Qp} ∅ ∗ x.1 ⟸?{x.2} ∅)).
 Proof.
   iIntros "?". iIntros.
-  iMod (stack_free with "[$] [$]") as "(? & (? & ? & [%vs ?]))".
+  iMod (stack_free with "[$] [$]") as "(? & (? & ? & [%vs ?]))". eauto.
   rewrite fmap_length. iFrame. iModIntro.
   iApply soup_mixer. iFrame.
 Qed.
