README.md
@@ -1,7 +1,6 @@
-# IrisFit
+# Will it Fit?
 
-An Iris instance for establishing heap space bounds of concurrent
-programs in the presence of garbage collection.
+A Lambda-Calculus with GC, equipped with a Separation Logic.
 
 ## Setup & build
 
@@ -11,8 +10,7 @@ dependencies, and build the project.
 Please allow at least 30 minutes for the installation and build to
 run.
 
-After the setup is done,
-you can manually build the project with `make` or `dune build`.
+To manually build the project, run `make` or `dune build`.
 
 ## Architecture
 
@@ -22,183 +20,25 @@ The architecture is as follows:
 * `spacelang/` for (almost not modified) files from
   [SpaceLang](https://gitlab.inria.fr/fpottier/diamonds/), taken with
   the authorization of the authors.
-* `language/` for the syntax of LambdaFit and the "oblivious" semantics of the
+* `language/` for the syntax & "oblivious" semantics of the
   language.
-* `final/` for the "default" semantics of LambdaFit and associated results.
+* `final/` for the "main" semantics and associated results.
 * `program_logic/` for program logic.
-* `sequential/` for the sequential mode presented
-  in [A High-Level Separation Logic for Heap Space under Garbage
-  Collection](https://dl.acm.org/doi/10.1145/3571218), which we emulate
-  in IrisFit.
+* `sequential/` for the emulation of the sequential mode presented
+in [A High-Level Separation Logic for Heap Space under Garbage Collection](https://doi.org/10.5281/zenodo.7129302).
 * `examples/` for various examples.
 
-## Link with the Paper
+## Links with Publications
 
-All the development is made with Weakest Preconditions (WP) rather
-than triples.
-Code pointers are expressed with notation µ λ and application of terms
-u and v as (u v).
-Closure creation uses the syntax `mk_clo` and closure call the syntax
-`call_clo`.
-Code pointers must contain no locations. The syntax does not actually
-enforce this constraint, so a side-condition locs(t) = ∅ appears from
-time to time.
-Moreover, while the paper assumes a global constant `S` describing the
-maximum size of the heap, we explicitly parameterize here predicates
-and lemmas with a variable (ms:nat).
+We present a correspondence between this formalization and related
+papers.
 
-### Figures
-
-* Figure 3 (LambdaFit: syntax):
-file `language/syntax.v`
-* Figure 4 (The head reduction relation):
-file `language/head_semantics.v`
-We define a relation `head_step` that covers every case, except for
-`fork`
-We then define a relation `head_step_conc`, which is either `fork`, or
-a `head_step`
-* Figure 5 (The step relation):
-file `language/semantics.v`
-The `step` relation is named `atomic_step`
-* Figure 6 (The garbage collection relation):
-file `final/gc.v`
-* Figure 7 (The action relation):
-file `final/final_semantics.v`
-* Figure 8 (Enabled actions (and auxiliary predicates)):
-file `final/final_semantics.v`
-The predicate `AllOut` is defined in file
-`program_logic/wp_adequacy.v`
-* Figure 9 (The main reduction relation):
-file `final/final_semantics.v`
-* Figure 10 (Structural reasoning rules):
-directory `program_logic/`
-  + Consequence: file `wp_updates.v`, lemma `wp_consequence`
-  + Frame: file `wp.v`, lemma `wp_frame`
-* Figure 11 (Reasoning rules of the “sizeof ” assertion):
-file `program_logic/mapsto.v`
-  + SizeOfPointsTo: `mapsto_extract_size_paper`
-  + SizeOfConfront: `sizeof_confront`
-  + SizeOfPersist: `sizeof_persist`
-* Figure 12 (Reasoning rules for space credits):
-file `program_logic/interp_base.v`
-  + ZeroSC: `diamonds_zero`
-  + SplitJoinSC: `diamond_split_iff`
-* Figure 13 (Reasoning rules for the pointed-by-heap assertion):
-file `program_logic/ph.v`
-  + JoinPBHeap: `mapsfrom_join`
-  + SplitPBHeap: `mapsfrom_split`
-  + CovPBHeap: `mapsfrom_weak_paper`
-* Figure 14 (Reasoning rules for the pointed-by-thread assertion):
-directory `program_logic/`
-  + FracPBThread: in file `pbt.v`, lemma `frac_pbt`
-  + CovPBThread: in file `pbt.v`, lemma `pbt_approx`
-  + TrimPBThread: in file `wp_clean`, lemma `supd_clean`
-* Figure 15 (Reasoning rules for “inside” and “outside” assertions):
-directory `program_logic/`
-  + InsideNotOutside: in file `wp_protected.v`, lemma
-    `inside_not_outside`
-  + AddTemporary: in file `wp_clean.v`, lemma `tupd_clean_debt`
-  + RemTemporary: in file `wp_clean.v`, lemma `debt_transfer`
-  + TrimInside: in file `wp_protected.v`, lemma `inside_clean`
-* Figure 16 (Reasoning rules for deallocation witnesses):
-file `program_logic/more_interp.v`
-  + CleanPBHeap: `mapsfrom_cleanup0`
-  + DeadPBHeap: `confront_mapsfrom_dag`
-  + DeadPBThread: `confront_pbt_dag`
-  + NoDanglingRootOut: `no_dangling_pointer`
-  + NoDanglingRootIn: `no_dangling_pointer_inside`
-  + DeadPersist: `persistent_dagger`
-* FreeOne: in file `program_logic/wp_free.v`, lemma `interp_free`
-* Figure 17 (Syntax-directed reasoning rules, without protected-section-specific rules and without Bind):
-directory `program_logic/`
-  + IfTrue, IfFalse: in file `wp.v`, lemma `wp_if`
-  + LetVal: in file `wp.v`, lemma `wp_let_val`
-  + Prim: in file `wp_call_prim.v`, lemma `wp_call_prim`
-  + CallPtr : in file `wp_call.v`, lemma `wp_call`
-  + Poll: in file `wp_poll.v`, lemma `wp_poll`
-  + Alloc: in file `wp_alloc.v`, lemma `wp_alloc`
-  + Load: in file `wp_load.v`, lemma `wp_load`
-  + Store: in file `wp_store.v`, lemma `wp_store`
-  + CASSuccess: in file `wp_cas.v`, lemma `wp_cas_suc`
-  + CASFailure: in file `wp_cas.v`, lemma `wp_cas_fail`
-  + Fork: in file `wp_fork.v` lemma `wp_fork`
-  + Val: in file `wp.v`, lemma `wp_val`
-* Figure 18 (Reasoning rules: protected-section-specific rules):
-directory `program_logic/`
-  + Enter: in file `wp_protected.v`, lemma `wp_enter`
-  + Exit: in file `wp_protected.v`, lemma `wp_exit`
-  + LoadInside: in file `wp_load.v`, lemma `wp_load_inside`
-  + StoreDead: in file `wp_store.v`, lemma `wp_store_dead`
-  + CASSuccessDead: in file `wp_cas.v`, lemma `wp_cas_suc_dead`
-* Figure 19 (Reasoning rules: the Bind rule):
-file `program_logic/wp.v`
-  + Bind: `wp_bind`
-* Figure 20 (Reasoning rules: additional mode-specific rules):
-file `program_logic/wp.v`
-  + SwitchMode: `wp_noclean`
-  + BindNoTrim: `wp_bind_noclean`
-* Figure 21 (Reasoning rules: logical deallocation):
-file `program_logic/wp_free.v`
-  + CloudEmpty: `ocloud_empty`
-  + CloudAdd: `ocloud_add`
-  + CloudFree: `supd_free_ocloud`
-* Figure 22 (Predicates used in the statement of the safety theorem):
-directory `final/`
-  + NotStuckVal, NotStuckStep: `final_semantics.v`
-  + Safe: `final_semantics.v`
-  + Always: `temporal_logic.v`
-* Figure 23 (Predicates used in the statement of the liveness theorem):
-file `final/temporal_logic.v`
-* Figure 24 (The oblivious reduction relation and associated predicates):
-  + InterleaveOblivious: file `final/final_semantics.v`, lemma `step_oblivious_alt`
-  + NotStuckObliviousVal,NotStuckObliviousStep: file `program_logic/wp_adequacy.v`, definition `not_stuck`
-* Figure 25 (Closures: macros for closure construction and invocation):
-file `language/closure.v`
-* Figure 26 (Closures: low-level API):
-file `program_logic/wp_closure.v`
-  + MkClo: `wp_mk_clo`
-  + CallClo: `wp_call_clo`
-  + CloFree: `closure_free`
-  + CloPersist: `Closure_persistent`
-* Figure 27 (Definition of the predicate Closure):
-file `program_logic/wp_closure.v`
-* Figure 28 (Closures: high-level API):
-file `program_logic/wp_spec.v`
-  + MkSpec: `wp_mk_spec`
-  + CallSpec: `wp_call_spec`
-  + SpecWeak: `spec_weak`
-  + SpecFree: `spec_free`
-  + SpecPersist: `Spec_persistent`
-* Figure 29 (Definition of the predicate Spec):
-file `program_logic/wp_spec.v`
-* Figure 30 (Key reasoning rules for triples with souvenir):
-file `program_logic/wp_spec.v`
-  + BindWithSouvenir: lemma `wpc_bind`
-  + AddSouvenir: lemma `wpc_context_singleton.v`
-  + ForgetSouvenir: lemma `wpc_weak`
-* Figure 31 (Definition of triples with souvenir):
-file `wpc.v`
-* Definition of atomic triples:
-file `program_logic/wpc_logatom.v`
-* Figure 32 (Code and specification of fetch-and-add):
-file `examples/toolbox/faa.v`
-* Figure 33 (Code and specification of a concurrent monotonic counter):
-file `examples/counter/counter.v`
-* Figure 34 (Code and specification of an async/finish library):
-file `examples/toolbox/async_finish.v`
-* Figure 35 (Specification of Treiber’s Stack):
-file `examples/lockfree/treiber.v`
-
-## Lemmas and Theorems
-
-| Result          | File                          | Name                         |
-|-----------------|-------------------------------|------------------------------|
-| Lemma 4.1       | `final/final_theorems.v`      | `EveryAllocFits_all_enabled` |
-| Lemma 4.2       | `final/final_theorems.v`      | `step_main_preserves_size`   |
-| Theorem 7.1     | `final/final_theorems.v`      | `wp_safety`                  |
-| Theorem 7.2 (1) | `final/final_theorems.v`      | `wp_safety_addpp`            |
-| Theorem 7.2 (2) | `final/final_theorems.v`      | `wp_liveness_addpp`          |
-| Theorem 7.3     | `program_logic/wp_adequacy.v` | `wp_adequacy_core`           |
+* For the submitted paper "Will it Fit? Verifying Heap Space Bounds of
+  Concurrent Programs under Garbage Collection with Separation Logic",
+  see `README_paper`.
+* For the PhD thesis of Alexandre Moine, "Formal Verification of Heap
+  Space Bounds under Garbage Collection",
+  see `README_thesis`.
 
 ## ProofGeneral
 
